theories/L/Complexity/Reductions/TMGenNP/M_LM2TM.v
@@ -1,0 +1,42 @@
+From Undecidability.L.Complexity Require Import NP.
+From Undecidability.TM Require TM ProgrammingTools CaseList.
+From Undecidability.TM Require Import TM SizeBounds.
+
+From Undecidability.L.Complexity  Require Import TMGenNP_fixed_mTM.
+
+From Undecidability.LAM Require HaltingProblem.
+From Undecidability.L.AbstractMachines Require Import FlatPro.Programs.
+     
+Unset Printing Coercions.
+From Coq.ssr Require ssrfun.
+Module Option := ssrfun.Option.
+
+From Coq Require Import Lia Ring Arith.
+
+From Undecidability.L.Complexity  Require Import GenNP_is_hard LMGenNP TMGenNP_fixed_mTM.
+Check fun M =>
+  restrictBy (LMHaltsOrDiverges Pro) (LMGenNP Pro) ⪯p (restrictBy (HaltsOrDiverges_fixed_mTM M) (TMGenNP_fixed_mTM M)).
+
+Module LMtoTM.
+  Module LAM := LAM.TM.HaltingProblem.
+  Section sec.
+    Import ProgrammingTools Combinators.
+
+    Check HaltingProblem.Loop.
+    
+    Context (sig F:finType) (n:nat) (M__multi : pTM sig F n).
+
+    (*TODO: Check that tape contaisn Encoding of programm*)
+(*
+    Definition M : pTM _ _ 12 := LiftTapes HaltingProblem.Loop [|Fin1,Fin2,|].
+
+    Definition Rel : pRel ((sigList (sigTape sig)) ^+) (option F) 1 :=
+      fun t '(y,t') => match y with
+                      None => ~ exists (v : tapes sig n), StepTM.contains_tapes t[@Fin0] v
+                    | Some y => exists (v v': tapes sig n), StepTM.contains_tapes t[@Fin0] v
+                                                      /\ StepTM.contains_tapes t'[@Fin0] v'
+                                                      /\ Canonical_Rel M__multi v (y,v')
+                    end.
+*)
+  End sec.
+End LMtoTM.
