theories/L/TM/CompCode.v
@@ -1,0 +1,98 @@
+
+From Undecidability.L Require Import LTactics LBool GenEncode Datatypes.Lists TMEncoding.
+From Undecidability.TM Require Import CodeTM Single.EncodeTapes.
+  
+Run TemplateProgram (tmGenEncode "boundary_enc" boundary).
+Hint Resolve boundary_enc_correct : Lrewrite.
+
+Lemma size_boundary (l:boundary):
+  L.size (enc l) = match l with START => 6 | STOP => 5 | UNKNOWN => 4 end.
+Proof.
+  change (enc l) with (boundary_enc l). 
+  destruct l;easy.
+Qed.
+
+Section sigList.
+  Context (sig : Type) `{H:registered sig}.
+  Run TemplateProgram (tmGenEncode "sigList_enc" (sigList sig)).
+
+  Global Instance term_sigList_X : computableTime' (@sigList_X sig) (fun _ _ => (1,tt)).
+  Proof. extract constructor. solverec.
+  Qed.
+
+  
+
+  Lemma size_sigList (l:sigList sig):
+    L.size (enc l) = match l with sigList_X x => L.size (enc x) + 7 | sigList_nil => 5 | _ => 4 end.
+  Proof.
+    change (enc l) with (sigList_enc l).
+    destruct l. all:cbn [sigList_enc map sumn size].
+    change ((match _ with
+             | @mk_registered _ enc _ _ => enc
+             end s)) with (enc s).
+    all:cbn;nia. 
+  Qed.
+
+
+End sigList.
+Hint Resolve sigList_enc_correct : Lrewrite.
+
+
+Section sigTape.
+  Context (sig : Type) `{H:registered sig}.
+  Run TemplateProgram (tmGenEncode "sigTape_enc" (sigTape sig)).
+
+  Global Instance term_LeftBlank_X : computableTime' (@LeftBlank sig) (fun _ _ => (1,tt)).
+  Proof. extract constructor. solverec. Qed.
+
+  Global Instance term_RightBlank_X : computableTime' (@RightBlank sig) (fun _ _ => (1,tt)).
+  Proof. extract constructor. solverec. Qed.
+
+  Global Instance term_MarkedSymbol_X : computableTime' (@MarkedSymbol sig) (fun _ _ => (1,tt)).
+  Proof. extract constructor. solverec. Qed.
+
+  Global Instance term_UnmarkedSymbol_X : computableTime' (@UnmarkedSymbol sig) (fun _ _ => (1,tt)).
+  Proof. extract constructor. solverec. Qed.
+
+  
+  Lemma size_sigTape (l:sigTape sig):
+    L.size (enc l) =
+    match l with
+      LeftBlank b => 11+ L.size (enc b)
+    | RightBlank b => 10+ L.size (enc b)
+    | NilBlank => 8
+    | MarkedSymbol x => 8 + L.size (enc x)
+    | UnmarkedSymbol x => 7 + L.size (enc x)
+    end.
+  Proof.
+    change (enc l) with (sigTape_enc l).
+    destruct l. all:cbn [sigTape_enc map sumn size].
+    1-2:unfold enc;cbn.
+    4-5:change ((match _ with
+             | @mk_registered _ enc _ _ => enc
+             end s)) with (enc s).
+    all:cbn;try nia.
+  Qed.
+
+  
+
+End sigTape.
+Hint Resolve sigTape_enc_correct : Lrewrite.
+
+Section encTape.
+  Context X `{registered X}.  
+  Definition _term_encode_tape : 
+    { time : UpToC (fun l => sizeOfTape l + 1)
+             &   computableTime' (@encode_tape X) (fun l _ => (time l,tt))}.
+  Proof.
+    evar (c1:nat).
+    exists_UpToC (fun l => c1 * sizeOfTape l + c1).
+    {  extract. recRel_prettify. solverec.
+       all:try rewrite !map_time_const. all:autorewrite with list. all:cbn [length].
+       all: ring_simplify. [c1]:exact 42. all:subst c1;nia. }
+    smpl_upToC_solve.
+  Qed.
+
+  Global Instance term_encode_tape : computableTime' (@encode_tape X) _ := projT2 _term_encode_tape.
+
+End encTape.
