theories/TM/MultiUnivTimeSpaceSimulation.v
@@ -530,14 +530,15 @@ Section U.
   Existing Instance retr_sigSimTape_sigUniv.
   Definition Univ : pTM sigUniv unit 6 := @Univ sigM sigUniv' retr_sigSimGraph_sigUniv retr_sigSimTape_sigUniv.
 
+  (*
   Check Univ : pTM sigUniv unit 6.
   Check Univ : pTM sigUniv'^+ unit 6.
-
+*)
 
   (** The single-tape version of [Univ] for alphabet [sigM] *)
   Definition U := ToSingleTape Univ.
   Definition sigU := ltac:(lazymatch type of U with pTM ?sigU _ _ => exact sigU end).
-  Check U : pTM sigU unit 1.
+(*  Check U : pTM sigU unit 1. *)
 
 
   (*
@@ -676,10 +677,10 @@ Section U.
   (** Because the asymtopic behaviour of [fp] only depends on the size of the tapes, we will just insert bogus tapes with the corresponding tapes size. *)
   Definition f (M : mTM sigM 1) : nat * nat -> nat := fun '(k, s) => fp M (bogus_tape s) k.
 *)
-
+(*
   Check (projT1 U) : mTM sigU 1.
   Check forall (tp tp' : tape sigU), terminates (projT1 U) [|tp|] 42 [|tp'|].
-
+*)
   (** [fp] is literally only another definition for [U_steps] *)
   Lemma fp_eq : forall M (T : tape sigM) k, fp M T k = U_steps (makeUnivTapes _ _ M T) (start M) T k.
   Proof. intros. reflexivity. Qed.
@@ -832,7 +833,7 @@ Section U.
 
 
   (** We only do space-analysis for [Univ] now, because the size of the [sigU] tapes is directly determined by the tapes of [Univ] *)
-  Check UnivSpaceBounds.Univ_size_nice'.
+  (* )Check UnivSpaceBounds.Univ_size_nice'. *)
 
 
   (* TODO: Maybe simplify this space bound a bit: every tape of [Univ], except the object tape, is bounded by a constant (that depends on M). *)
@@ -887,7 +888,7 @@ Section MakeSingleTape_Bounded_by_sizeOfmTapes.
   Variable (sig : finType) (n : nat).
 
   (** We've already proven that [sizeOfTape (makeSingleTape T)] is the sum of the tape sizes (plus some constant) *)
-  Check makeSingleTape_sizeOfTape.
+  (* )Check makeSingleTape_sizeOfTape. *)
 
   Lemma tam (T : tapes sig n) :
     max_list_map (fun t : tape sig => Encode_tape_size t + 1) (vector_to_list T) <= sizeOfmTapes T + 3.
@@ -969,7 +970,7 @@ Section UnivMultiTimeSpaceTheorem.
 
   Notation pM' := (ToSingleTape pM).
   Notation M' := (projT1 pM').
-  Check M' : mTM sigM' 1.
+  (* )Check M' : mTM sigM' 1. *)
 
   Notation "'castState' q" := (q : (states (projT1 pM))) (at level 1).
 
@@ -1122,7 +1123,7 @@ Section UnivMultiTimeSpaceTheorem.
 
   (** Simplify [sizeOfTape (makeSingleTape T)] *)
 
-  Check makeSingleTape_sizeOfmTapes.
+  (* )Check makeSingleTape_sizeOfmTapes. *)
 
   Lemma Mfp_nice3 :
     {c : nat | forall (T : tapes sigM n) (k : nat),
@@ -1289,7 +1290,7 @@ Section UnivMultiTimeSpaceTheorem.
   Qed.
 
 
-  Print UnivSpaceBounds.Univ_size_bound.
+(*  Print UnivSpaceBounds.Univ_size_bound. *)
     
 
   (** We need to bound the size of the [sigMU] tape *)
@@ -1463,5 +1464,7 @@ Section UnivMultiTimeSpaceTheorem.
 
 End UnivMultiTimeSpaceTheorem.
 
+(*
 Print Assumptions EndTheorem1.
 Print Assumptions EndTheorem2.
+*)
