theories/TM/PrettyBounds/SizeBounds.v
@@ -1,7 +1,7 @@
 
             
 From Undecidability Require Import MaxList.
-From Undecidability Require Import TM.TM.
+From Undecidability Require Import TM.TM TM.Code.CodeTM.
 
 (* MOVE : this file contains general lemmas from is all over the place... *)
 
@@ -88,6 +88,42 @@ Proof.
       * now constructor; auto.
 Qed.
 
+(*MOVE*)
+Lemma list_eq_nth_error X (xs ys : list X) :
+  (forall n, nth_error xs n = nth_error ys n) -> xs = ys.
+Proof.
+  induction xs in ys|-*;destruct ys;cbn;intros H. 1:easy. 1-2:now specialize (H 0).
+  generalize (H 0).  intros [= ->]. erewrite IHxs. easy. intros n'. now specialize (H (S n')).
+Qed.
+
+Lemma vector_nth_error_nat X n' i (xs : Vector.t X n') :
+  nth_error (Vector.to_list xs) i = match lt_dec i n' with
+                                      Specif.left H => Some (Vector.nth xs (Fin.of_nat_lt H))
+                                    | _ => None
+                                    end.
+Proof.
+  clear. rewrite <- vector_to_list_correct. induction xs in i|-*. now destruct i.
+  cbn in *. destruct i;cbn. easy. rewrite IHxs. do 2 destruct lt_dec. 4:easy. now symmetry;erewrite Fin.of_nat_ext. all:exfalso;nia. 
+Qed.
+
+
+Lemma vector_nth_error_fin X n' i (xs : Vector.t X n') :
+  nth_error (Vector.to_list xs) (proj1_sig (Fin.to_nat i)) = Some (Vector.nth xs i).
+Proof.
+  clear. rewrite <- vector_to_list_correct. induction xs in i|-*. now inv  i. cbn;rewrite vector_to_list_correct in *.
+  cbn in *. edestruct (fin_destruct_S) as [ (i'&->)| -> ]. 2:now cbn.
+  unshelve erewrite (_ : Fin.FS = Fin.R 1). reflexivity.
+  setoid_rewrite (Fin.R_sanity 1 i'). cbn. easy.
+Qed.
+
+
+Lemma vector_app_to_list X k k' (xs : Vector.t X k) (ys : Vector.t X k'):
+  vector_to_list (Vector.append xs ys) = vector_to_list xs ++ vector_to_list ys.
+Proof.   
+  induction xs. easy. cbn. congruence.
+Qed.
+
+
 Lemma sizeOfmTapes_upperBound (sig : Type) (n : nat) (tps : tapes sig n) :
   forall t, Vector.In t tps -> sizeOfTape t <= sizeOfmTapes tps.
 Proof. intros. rewrite sizeOfmTapes_max_list_map. apply max_list_map_ge. now apply vector_to_list_In. Qed.
@@ -99,3 +135,23 @@ Proof.
   unfold max_list.
   induction l;cbn. 2:rewrite max_list_rec_max'. all:nia.
 Qed.
+
+
+Lemma right_sizeOfTape sig' (t:tape sig') :
+  length (right t) <= sizeOfTape t.
+Proof.
+  destruct t;cbn. all:autorewrite with list;cbn. all:nia.
+Qed.
+
+Lemma size_list X sigX (cX: codable sigX X) (l:list X) :
+  size _ l = sumn (map (size cX) l) + length l + 1.
+Proof.
+  unfold size. cbn. rewrite encode_list_concat.
+  rewrite app_length, length_concat, map_map. cbn.
+  change S with (fun x => 1 + x). rewrite sumn_map_add,sumn_map_c. setoid_rewrite map_length.
+  cbn.  nia.
+Qed.
+
+Lemma destruct_vector1 (X : Type) (v : Vector.t X 1) :
+  exists x, v = [| x |].
+Proof. destruct_vector. eauto. Qed.
